Imp/StackMachine/Structural.lean
@@ -3,22 +3,22 @@ import Mathlib.Data.List.Defs
 
 inductive Instr.Step: Instr × StackMachine → StackMachine → Prop where
   | loadi₁:
-    Step (loadi n, ⟨pc, s, stk⟩) ⟨pc + 1, s, stk.concat n⟩
+    Step (loadi n, ⟨pc, s, stk⟩) ⟨pc + 1, s, n::stk⟩
 
   | load₁:
-    Step (load x, ⟨pc, s, stk⟩) ⟨pc + 1, s, stk.concat $ s x⟩
+    Step (load x, ⟨pc, s, stk⟩) ⟨pc + 1, s, (s x)::stk⟩
 
-  | add₁ (h: [a, b] = stk.take 2):
-    Step (add, ⟨pc, s, stk⟩) ⟨pc + 1, s, stk.tail.tail.concat $ a + b⟩
+  | add₁ (h: a::b::t = stk):
+    Step (add, ⟨pc, s, stk⟩) ⟨pc + 1, s, (a + b)::t⟩
 
-  | store₁ (h: some head = stk.head?):
-    Step (store x, ⟨pc, s, stk⟩) ⟨pc + 1, s⟪x ≔ head⟫, stk.tail⟩
+  | store₁ (h: a::t = stk):
+    Step (store x, ⟨pc, s, stk⟩) ⟨pc + 1, s⟪x ≔ a⟫, t⟩
 
   | jmp₁:
     Step (jmp n, ⟨pc, s, stk⟩) ⟨pc + 1 + n, s, stk⟩
 
-  | jmplt₁ (h: [a, b] = stk.take 2):
+  | jmplt₁ (h: a::b::t = stk):
     Step (jmplt n, ⟨pc, s, stk⟩) ⟨bif b < a then pc + 1 + n else pc + 1, s, stk⟩
 
-  | jmpge₁ (h: [a, b] = stk.take 2):
+  | jmpge₁ (h: a::b::t = stk):
     Step (jmpge n, ⟨pc, s, stk⟩) ⟨bif b ≥ a then pc + 1 + n else pc + 1, s, stk⟩
